***
_Solution:_ 

a. The mean of the negative binomial (in this formulation) is 
$$
E(Y) = \frac{(1-p)k}{p}.
$$

Equating to the empirical mean, we have 
$$
\frac{(1-p)r}{p} = \bar{y}
$$ 
therefore 
$$
\hat{p}_{MM}= \frac{r}{\bar{y} + r}.
$$

b. The log-likelihood is 
$$
l(p|\mathbf{y},k) = \sum_{i=1}^{n} \log \left(\frac{\Gamma(k+y_{i})}{y_{i}!~\Gamma(k)}p^{k} (1-p)^{y_{i}} \right)
$$
which can be simplified to
$$
l(p|\mathbf{y},k) = C(k,\boldsymbol{y}) + n k \log p + \sum_{i=1}^{n}y_{i} \log (1 - p)
$$
where 
$$
C(k,\mathbf{y}) = \sum_{i=1}^{n} \log \left(\frac{\Gamma(k+y_{i})}{y_{i}!~\Gamma(k)}\right)
$$ 
does not depend on $p$.  

Setting $\frac{\partial l}{\partial p} = 0$
$$
\frac{\partial l}{\partial p} = \frac{nk}{p} - \frac{\sum_{i=1}^{n}y_{i}}{1-p}
$$

$$
0=\frac{nk}{p} - \frac{\sum_{i=1}^{n}y_{i}}{1-p}
$$
$$
\hat{\theta}_{ML} = \frac{k}{\bar{y} + k}
$$

c. The MM and MLE are the same.
***
