
***
*Solution*: 

The least squares optimisation can be found by solving

$$
\min_{b} \sum_{i=1}^{n}\left(y_{i} - b x_{i}^2\right)^{2}
$$

Let 
$$
r(b) = \sum_{i=1}^{n}(y_{i} - b x_{i}^2)^{2}
$$ 
then
$$
\frac{\partial r}{\partial b} = -2 \sum_{i=1}^{n}x_{i}^2(y_{i} - b x_{i}^2)
$$
$$
\phantom{\frac{\partial r}{\partial b}}= -2 \left(\sum_{i=1}^{n}x_{i}^2 y_{i} - b\sum_{i=1}^{n}x_{i}^4\right)
$$

Setting $\frac{\partial r}{\partial b} = 0$ results in 

$$
\hat{b}_{LS} = \frac{\sum_{i=1}^{n}x_{i}^2y_{i}}{\sum_{i=1}^{n}x_{i}^4}
$$

***